DistributedSystems/VerifiedDS/src/Dafny/Distributed/Protocol/CausalMesh/proof/meta_is_met.dfy
@@ -1,0 +1,134 @@
+include "../distributed_system.dfy"
+// include "causalcut.dfy"
+include "packet_sending.dfy"
+include "properties.dfy"
+include "propagation.dfy"
+include "../../../Common/Collections/Seqs.s.dfy"
+
+module CausalMesh_Proof_MetaIsMet_i {
+import opened CausalMesh_Cache_i
+import opened CausalMesh_Message_i
+import opened CausalMesh_Types_i
+import opened Environment_s
+import opened CausalMesh_DistributedSystem_i
+import opened CausalMesh_Properties_i
+import opened CausalMesh_Proof_Actions_i
+import opened Temporal__Temporal_s
+import opened CausalMesh_proof_Assumptions_i
+import opened CausalMesh_Proof_Constants_i
+import opened CausalMesh_Proof_PropagationLemma_i
+import opened CausalMesh_Proof_Propagation_i
+import opened CausalMesh_Proof_PacketSending_i
+import opened CausalMesh_Proof_Properties_i
+// import opened CausalMesh_Proof_MessageReadReply_i
+import opened Collections__Seqs_s
+import opened Collections__Maps_i
+import opened Collections__Maps2_s
+
+lemma lemma_MetaIsMetImpliesItsDepsAreMet(
+    b:Behavior<CMState>,
+    i:int,
+    meta:Meta
+)
+    requires 0 < i 
+    requires IsValidBehaviorPrefix(b, i)
+    requires forall j :: 0 <= j < i ==> CMNext(b[j], b[j+1])
+    requires MetaValid(meta)
+    requires AVersionIsMetOnAllServers(b, i, meta.key, meta.vc)
+    requires forall j :: 0 < j <= i ==> AllWriteDepsAreMet(b, j)
+    ensures AllVersionsInDepsAreMetOnAllServers(b, i, meta.deps)
+{
+     if i <= 1 {
+        assert CMNext(b[i-1], b[i]);
+        lemma_MetaIsMetImpliesItsDepsAreMetForIndexOne(b, i, meta);
+        return;
+    }
+
+    assert 0 < i - 1;
+
+    lemma_ConstantsAllConsistent(b, i-1);
+    lemma_ConstantsAllConsistent(b, i);
+
+    lemma_BehaviorValidImpliesOneStepValid(b, i);
+
+    if AVersionIsMetOnAllServers(b, i-1, meta.key, meta.vc)
+    {
+        lemma_MetaIsMetImpliesItsDepsAreMet(b, i-1, meta);
+        lemma_DepsAreMetAreTransitive(b, i, meta);
+        return;
+    }
+
+    // var ios := lemma_ActionThatChangesServerIsThatServersAction(b, i, )
+    
+    // how to find the node that is the tail of propagation of meta?
+
+    var ios:seq<CMIo>;
+    var idx :| 0 <= idx < Nodes;
+
+    assert CMNext(b[i-1], b[i]);
+    assert 0 < i; 
+    assert IsValidBehaviorPrefix(b, i);
+    assert MetaValid(meta);
+    assert 0 <= idx < Nodes;
+
+    lemma_IosIsPropagationTail(b, i, idx, ios, meta);
+
+    assert ReceivePropagate(b[i-1].servers[idx].s, b[i].servers[idx].s, ios[0].r, ExtractSentPacketsFromIos(ios));
+
+    var p_pro := ios[0].r;
+    assert p_pro.dst == idx;
+
+    lemma_PropagationAtTail2(b, i, idx, p_pro, ios);
+    assert AllVersionsInDepsAreMetOnAllServers(b, i, p_pro.msg.meta.deps);
+    assert AllVersionsInDepsAreMetOnAllServers(b, i, meta.deps);
+}
+
+lemma {:axiom} lemma_MetaIsMetImpliesItsDepsAreMetForIndexOne(
+    b:Behavior<CMState>,
+    i:int,
+    meta:Meta
+)
+    requires i == 1 
+    requires IsValidBehaviorPrefix(b, i)
+    requires CMNext(b[i-1], b[i])
+    requires MetaValid(meta)
+    ensures !exists p :: p in b[i].environment.sentPackets && p.msg.Message_Propagation?
+    ensures AllVersionsInDepsAreMetOnAllServers(b, i, meta.deps)
+
+lemma {:axiom} lemma_DepsAreMetAreTransitive(
+    b:Behavior<CMState>,
+    i:int,
+    meta:Meta
+)
+    requires i > 1 
+    requires IsValidBehaviorPrefix(b, i)
+    requires CMNext(b[i-1], b[i])
+    requires MetaValid(meta)
+    requires AllVersionsInDepsAreMetOnAllServers(b, i-1, meta.deps)
+    ensures AllVersionsInDepsAreMetOnAllServers(b, i, meta.deps)
+// {
+
+// }
+
+lemma {:axiom} lemma_IosIsPropagationTail(
+    b:Behavior<CMState>,
+    i:int,
+    idx:int,
+    ios:seq<CMIo>,
+    meta:Meta
+)
+    requires 0 < i 
+    requires IsValidBehaviorPrefix(b, i)
+    requires CMNext(b[i-1], b[i])
+    requires MetaValid(meta)
+    requires 0 <= idx < Nodes
+    ensures |ios| > 1
+    ensures ios[0].LIoOpReceive?
+    ensures ios[0].r.msg.Message_Propagation?
+    ensures ios[0].r in b[i-1].environment.sentPackets
+    ensures ReceivePropagate(b[i-1].servers[idx].s, b[i].servers[idx].s, ios[0].r, ExtractSentPacketsFromIos(ios))
+    ensures ios[0].r.msg.start == b[i-1].servers[idx].s.next
+    ensures ios[0].r.dst == idx
+    ensures ios[0].r.msg.meta == meta
+    // ensures forall j :: 0 < j <= i ==> AllWriteDepsAreMet(b, j)
+}
